\section[Äquivalenz mit XOR]{Wie zeigen Sie, die Äquivalenz der folgenden Ausdrücke mit XOR}
(x\vee y)\wedge \neg(x\wedge y)\\
\begin{tabular}[h]{c|c|c|c|c}
	x & y & (x\vee y) & \neg(x\wedge y) & a\wedge b \\
	\hline
	0 & 0 & 0 & 1 & 0 \\
	0 & 1 & 1 & 1 & 1 \\
	1 & 0 & 1 & 1 & 1 \\
	1 & 1 & 1 & 0 & 0 \\
\end{tabular}\\
\neg((x\wedge y)\vee(\neg x\wedge \neg y))\\
\begin{tabular}[h]{c|c|c|c|c}
	x & y & (x\wedge y) & (\neg x\wedge \neg y) & \neg(a\vee b) \\
	\hline
	0 & 0 & 0 & 1 & 0 \\
	0 & 1 & 0 & 0 & 1 \\
	1 & 0 & 0 & 0 & 1 \\
	1 & 1 & 1 & 0 & 0 \\
\end{tabular}\\
\neg(x\wedge y)\wedge(x\vee y)\\
\begin{tabular}[h]{c|c|c|c|c}
	x & y & \neg(x\wedge y) & (x\vee y) & a\wedge b \\
	\hline
	0 & 0 & 0 & 1 & 0 \\
	0 & 1 & 1 & 1 & 1 \\
	1 & 0 & 1 & 1 & 1 \\
	1 & 1 & 1 & 0 & 0 \\
\end{tabular}